progress

extra/LambdaSepSpecExtra.v
@@ -162,3 +162,176 @@ Proof using.
   { intros F. applys rule_extract_hprop. applys M. }
 Qed.
 
+
+================
+LIFTED
+
+
+
+
+(* ********************************************************************** *)
+(* * Bonus *)
+
+(* DEPRECATED?
+
+(* ---------------------------------------------------------------------- *)
+(** Reformulation of rule for N-ary functions *)
+
+Definition Spec_funs (xs:vars) (t1:trm) (F:val) :=
+  forall (Xs:dyns), length xs = length Xs ->
+    Triple (Substn xs Xs t1) ===> Triple (trm_apps F (encs Xs)).
+
+Lemma spec_funs_val_funs : forall xs t1,
+  var_distinct xs ->
+  xs <> nil ->
+  Spec_funs xs t1 (val_funs xs t1).
+Proof using. introv D N E M. applys* Triple_apps_funs. splits~. Qed.
+
+
+(* ---------------------------------------------------------------------- *)
+(** Reformulation of rule for N-ary recursive functions *)
+
+Definition Spec_fixs (f:var) (xs:vars) (t1:trm) (F:val) :=
+  forall (Xs:dyns), length xs = length Xs ->
+    Triple (subst1 f F (Substn xs Xs t1)) ===> Triple (trm_apps F (encs Xs)).
+
+Lemma Spec_fixs_val_fixs : forall f xs t1,
+  var_distinct (f::xs) ->
+  xs <> nil ->
+  Spec_fixs f xs t1 (val_fixs f xs t1).
+Proof using. introv D N L M. applys* Triple_apps_fixs. splits~. Qed.
+
+
+(* ---------------------------------------------------------------------- *)
+(** Functions of one argument *)
+
+(* TODO: upper case arguments that are encoded *)
+
+Lemma Triple_app_fun : forall x F V t1 H A `{EA: Enc A} (Q:A->hprop),
+  F = (val_fun x t1) ->
+  Triple (subst x V t1) H Q ->
+  Triple (trm_app F V) H Q.
+Proof using. introv EF M. applys* triple_app_fun. Qed.
+
+Definition Spec_fun (x:var) (t1:trm) (F:val) :=
+  forall X, Triple (subst x X t1) ===> Triple (trm_app F X).
+
+Lemma Spec_fun_val_fun : forall x t1,
+  Spec_fun x t1 (val_fun x t1).
+Proof using. introv. intros X H Q M. applys* Triple_app_fun. Qed.
+
+Lemma Triple_fun_spec : forall x t1 H (Q:func->hprop),
+  (forall (F:val), Spec_fun x t1 F -> H ==> Q F) ->
+  Triple (trm_fun x t1) H Q.
+Proof using.
+  introv M. forwards M': (rm M) (val_fun x t1).
+  { applys Spec_fun_val_fun. }
+  { applys~ Triple_fun. }
+Qed.
+
+Lemma Triple_let_fun : forall f x t1 t2 H A `{EA: Enc A} (Q:A->hprop),
+  (forall (F:val), Spec_fun x t1 F -> Triple (subst f F t2) H Q) ->
+  Triple (trm_let f (trm_fun x t1) t2) H Q.
+Proof using.
+  introv M. applys Triple_let (fun F => \[Spec_fun x t1 F] \* H).
+  { applys Triple_fun_spec. introv HF. hsimpl~. }
+  { intros F. applys Triple_extract_hprop. applys M. }
+Qed.
+
+(* ---------------------------------------------------------------------- *)
+(** Recursive functions of one argument *)
+
+Lemma Triple_app_fix : forall f x F V t1 H A `{EA: Enc A} (Q:A->hprop),
+  F = (val_fix f x t1) ->
+  Triple (subst f F (subst x V t1)) H Q ->
+  Triple (trm_app F V) H Q.
+Proof using. introv EF M. applys* triple_app_fix. Qed.
+
+Definition Spec_fix (f:var) (x:var) (t1:trm) (F:val) :=
+  forall X, Triple (subst f F (subst x X t1)) ===> Triple (trm_app F X).
+
+Lemma Spec_fix_val_fix : forall f x t1,
+  Spec_fix f x t1 (val_fix f x t1).
+Proof using. introv. intros X H Q M. applys* Triple_app_fix. Qed.
+
+Lemma Triple_fix_spec : forall f x t1 H (Q:func->hprop),
+  (forall (F:val), Spec_fix f x t1 F -> H ==> Q F) ->
+  Triple (trm_fix f x t1) H Q.
+Proof using.
+  introv M. forwards M': (rm M) (val_fix f x t1).
+  { applys Spec_fix_val_fix. }
+  { applys~ Triple_fix. }
+Qed.
+
+Lemma Triple_let_fix : forall f x t1 t2 H A `{EA: Enc A} (Q:A->hprop),
+  (forall (F:val), Spec_fix f x t1 F -> Triple (subst f F t2) H Q) ->
+  Triple (trm_let f (trm_fix f x t1) t2) H Q.
+Proof using.
+  introv M. applys Triple_let (fun F => \[Spec_fix f x t1 F] \* H).
+  { applys Triple_fix_spec. introv HF. hsimpl~. }
+  { intros F. applys Triple_extract_hprop. applys M. }
+Qed.
+
+
+(* ---------------------------------------------------------------------- *)
+(** Derived rules *)
+
+Lemma Triple_if' : forall t0 t1 t2 H (Q1:bool->hprop) A `{EA:Enc A} (Q:A->hprop),
+  Triple t0 H Q1 ->
+  Triple t1 (Q1 true) Q ->
+  Triple t2 (Q1 false) Q ->
+  Triple (trm_if t0 t1 t2) H Q.
+Proof using.
+  introv M0 M1 M2. applys* Triple_if. { intros b. case_if*. }
+Qed.
+
+Lemma Triple_let_val : forall A1 `{Enc A1} (V1:A1) x v1 t2 H A `{EA: Enc A} (Q:A->hprop),
+  v1 = enc V1 ->
+  (forall X, X = V1 -> Triple (Subst x (Dyn X) t2) H Q) ->
+  Triple (trm_let x (trm_val v1) t2) H Q.
+Proof using.
+  introv E M. applys triple_let_val. intros X EX. subst. applys~ M.
+Qed.
+
+*)
+
+(* ---------------------------------------------------------------------- *)
+(** Other rules for loops *)
+
+(*
+Lemma Triple_while : forall t1 t2 H Q,
+  (forall t,
+     (forall H' Q', triple (trm_if t1 (trm_seq t2 t) val_unit) H' Q' ->
+                    triple t H' Q') ->
+    triple t H Q) ->
+  triple (trm_while t1 t2) H Q.
+
+Lemma Triple_while_inv : forall (A:Type) (I:bool->A->hprop) (R:A->A->Prop) t1 t2 H,
+  let Q := (fun r => \exists Y, I false Y) in
+  wf R ->
+  (H ==> (\exists b X, I b X) \* \Top) ->
+  (forall t b X,
+      (forall b' X', R X' X -> triple t (I b' X') Q) ->
+      triple (trm_if t1 (trm_seq t2 t) val_unit) (I b X) Q) ->
+  triple (trm_while t1 t2) H Q.
+
+Lemma Triple_for_gt : forall x n1 n2 t3 H Q,
+  n1 > n2 ->
+  (fun r => \* H) ===> (Q \*+ \Top) ->
+  triple (trm_for x n1 n2 t3) H Q.
+
+Lemma Triple_for_le : forall Q1 x n1 n2 t3 H Q,
+  n1 <= n2 ->
+  triple (subst x n1 t3) H Q1 ->
+  triple (trm_for x (n1+1) n2 t3) (Q1 val_unit) Q ->
+  (forall v, ~ is_val_unit v -> (Q1 v) ==> \[False]) ->
+  triple (trm_for x n1 n2 t3) H Q.
+
+Lemma Triple_for_inv : forall (I:int->hprop) H' x n1 n2 t3 H Q,
+  (n1 <= n2+1) ->
+  (H ==> I n1 \* H') ->
+  (forall i, n1 <= i <= n2 ->
+     triple (subst x i t3) (I i) (fun r => I (i+1))) ->
+  (I (n2+1) \* H' ==> Q val_unit \* \Top) ->
+  triple (trm_for x n1 n2 t3) H Q.
+*)
