theories/LambdaSepLifted.v
@@ -24,15 +24,10 @@ Open Scope heap_scope.
 
 Implicit Types l : loc.
 Implicit Types u : unit.
-
-
-(* ********************************************************************** *)
-(* * Types *)
-
-(* ---------------------------------------------------------------------- *)
-(* ** Func type *)
-
-Definition func := val.
+Implicit Types z : bind.
+Implicit Types v : val.
+Implicit Types n : int.
+Implicit Types b : bool.
 
 
 (* ********************************************************************** *)
@@ -46,18 +41,6 @@ Class Enc (A:Type) :=
 
 Notation "`` V" := (enc V) (at level 8, format "`` V").
 
-
-(* TEMPORARY: this is patch of a TLC tactic to prevent undesired
-   eager instantiation of the typeclasses [Enc]. *)
-Ltac app_evar t A cont ::=
-  let x := fresh "TEMP" in
-  let T :=
-    match A with Enc ?X => constr:(id Enc X) | _ => constr:(A) end in
-  evar (x:T);
-  let t' := constr:(t x) in
-  let t'' := (eval unfold x in t') in
-  subst x; cont t''.
-
 (** Notation for lists of encoded values *)
 
 Notation "``[ ]" :=
@@ -69,6 +52,19 @@ Notation "``[ x , y , .. , z ]" :=
 
 Open Scope enc_scope.
 Delimit Scope enc_scope with enc.
+
+
+(** TEMPORARY: below is a patch for TLC tactics to prevent undesired
+   eager instantiation of the typeclasses [Enc]. *)
+
+Ltac app_evar t A cont ::=
+  let x := fresh "TEMP" in
+  let T :=
+    match A with Enc ?X => constr:(id Enc X) | _ => constr:(A) end in
+  evar (x:T);
+  let t' := constr:(t x) in
+  let t'' := (eval unfold x in t') in
+  subst x; cont t''.
 
 
 (* ---------------------------------------------------------------------- *)
@@ -110,6 +106,15 @@ Proof using. auto. Qed.
 
 
 (* ---------------------------------------------------------------------- *)
+(* ** Func type *)
+
+(** Let [func] be an alias for [val], used to describing functions. 
+    This type name helps deriving instances of encoders. *)
+
+Definition func := val.
+
+
+(* ---------------------------------------------------------------------- *)
 (* ** Encoder instances *)
 
 Global Instance Enc_dyn : Enc dyn.
@@ -138,29 +143,6 @@ Proof using. constructor. applys (fun (p:prim) => val_prim p). Defined.
 
 Global Opaque Enc_dyn Enc_loc Enc_unit Enc_bool Enc_int
               Enc_func Enc_val Enc_prim.
-
-
-(* ---------------------------------------------------------------------- *)
-(* ** Specification of encoders for dyns *)
-
-(* TODO: not needed? *)
-Lemma enc_dyn_eq' : forall (d:dyn),
-  enc d = dyn_to_val d.
-Proof using. auto. Qed.
-
-(* TODO: not needed? *)
-Lemma enc_dyn_eq : forall (d:dyn),
-  enc d = @enc _ (dyn_enc d) (dyn_value d).
-Proof using. auto. Qed.
-
-Lemma enc_dyn_make : forall `{EA:Enc A} (V:A),
-  enc (dyn_make V) = enc V.
-Proof using. auto. Qed.
-
-Hint Rewrite @enc_dyn_make : rew_enc_dyn.
-
-Tactic Notation "rew_enc_dyn" :=
-  autorewrite with rew_enc_dyn.
 
 
 (* ---------------------------------------------------------------------- *)
@@ -194,6 +176,20 @@ Lemma enc_prim_eq : forall (p:prim),
   enc p = p.
 Proof using. auto. Qed.
 
+(** Specification of encoders for values of type [dyn] *)
+
+Lemma enc_dyn_eq_dyn_to_val : forall (d:dyn),
+  enc d = dyn_to_val d.
+Proof using. auto. Qed.
+
+(** The encoding of a dynamic value [V] is the same as the encoding of V *)
+
+Lemma enc_dyn_make : forall `{EA:Enc A} (V:A),
+  enc (dyn_make V) = enc V.
+Proof using. auto. Qed.
+
+(** [rew_enc] normalizes all encoders. *)
+
 Hint Rewrite enc_dyn_make enc_loc_eq enc_unit_eq enc_bool_eq enc_int_eq
              enc_func_eq enc_val_eq enc_prim_eq : rew_enc.
 
@@ -203,6 +199,17 @@ Tactic Notation "rew_enc" "in" hyp(H) :=
   autorewrite with rew_enc in H.
 Tactic Notation "rew_enc" "in" "*" :=
   autorewrite with rew_enc in *.
+
+(** [rew_enc] normalizes only the [dyn] encoder. *)
+
+Hint Rewrite @enc_dyn_make : rew_enc_dyn.
+
+Tactic Notation "rew_enc_dyn" :=
+  autorewrite with rew_enc_dyn.
+Tactic Notation "rew_enc_dyn" "in" hyp(H) :=
+  autorewrite with rew_enc_dyn in H.
+Tactic Notation "rew_enc_dyn" "in" "*" :=
+  autorewrite with rew_enc_dyn in *.
 
 
 (* ---------------------------------------------------------------------- *)
@@ -215,7 +222,6 @@ Lemma Enc_injective_eq : forall `{EA:Enc A} (V1 V2:A),
   Enc_injective EA ->
   (enc V1 = enc V2) = (V1 = V2).
 Proof using. introv E. extens. iff M. { applys~ E. } { subst~. } Qed.
-
 
 Lemma Enc_injective_loc : Enc_injective Enc_loc.
 Proof using.
@@ -249,6 +255,7 @@ Hint Resolve Enc_injective_loc Enc_injective_unit Enc_injective_bool
 (** List of dyns *)
 
 Definition dyns := list dyn.
+
 (** Notation for lists of dynamic values *)
 
 Notation "``[ ]" :=
@@ -332,8 +339,13 @@ Qed.
 (* ---------------------------------------------------------------------- *)
 (* ** Lifting of postconditions *)
 
+(** [Post Q] converts a postcondition of type [A->hprop] into a
+    postcondition of type [val->hprop], where [A] is encodable. *)
+
 Definition Post A `{Enc A} (Q:A->hprop) : val->hprop :=
   fun v => \exists V, \[v = enc V] \* Q V.
+
+(** [Post] is covariant *)
 
 Lemma Post_himpl : forall `{Enc A} Q Q',
   Q ===> Q' ->
@@ -342,6 +354,8 @@ Proof using.
   introv M. unfold Post. intros v.
   hpull. intros x E. subst v. hsimpl*.
 Qed.
+
+(** [Post] distributes over the star *)
 
 Lemma Post_star : forall `{Enc A} Q H,
   Post (Q \*+ H) = (Post Q) \*+ H.
@@ -356,12 +370,13 @@ Local Hint Resolve Post_himpl.
 (* ---------------------------------------------------------------------- *)
 (* ** Lifting of heap predicates *)
 
-(** Singleton *)
+(** Singleton: [l ~~> V] describes a singleton heap at location [l]
+    with contents [V], where the value [V] has some encodable type [A]. *)
 
 Definition Hsingle `{EA:Enc A} (V:A) (l:loc) : hprop :=
   hsingle l (enc V).
 
-Notation "l '~~>' v" := (l ~> Hsingle v)
+Notation "l '~~>' V" := (l ~> Hsingle V)
   (at level 32, no associativity) : heap_scope.
 
 Lemma Hsingle_to_hsingle : forall `{EA:Enc A} (l:loc) (V:A),
@@ -374,15 +389,16 @@ Proof using. intros. xunfold Hsingle. applys hsingle_not_null. Qed.
 
 Arguments Hsingle_not_null : clear implicits.
 
-(** Field *)
+(** Field: [ l `.` f ~~> V ] describes the ownership of a record field
+    storing one encodable value [V]. *)
 
 Definition Hfield `{EA:Enc A} (V:A) (l_f:loc*field) : hprop :=
   let '(l,f) := l_f in
   hfield l f (enc V).
 
-Notation "l `.` f '~~>' v" := ((l,f) ~> Hfield v)
+Notation "l `.` f '~~>' V" := ((l,f) ~> Hfield V)
   (at level 32, f at level 0, no associativity,
-   format "l `.` f  '~~>'  v") : heap_scope.
+   format "l `.` f  '~~>'  V") : heap_scope.
 
 Lemma Hfield_eq_fun_Hsingle :
   @Hfield = (fun `{EA:Enc A} (V:A) l_f => let '(l,f) := l_f in ((l+f)%nat ~~> V) \* \[l <> null]).
@@ -406,8 +422,13 @@ Arguments Hfield_not_null : clear implicits.
 (* ---------------------------------------------------------------------- *)
 (* ** Lifting of substitution *)
 
-Definition Subst1 (y:var) (d:dyn) (t:trm) : trm :=
-  subst1 y (enc d) t.
+(** [Subst1 y d t] substitues variable [y] with the encoding of [V] in [t]. *)
+
+Definition Subst1 A `{EA:Enc A} (z:bind) (V:A) (t:trm) : trm :=
+  subst1 z (enc V) t.
+
+(** [Substn ys ds t] substitues the list of variables [ys] with the
+    encodings of the list of dynamic values [ds] in [t]. *)
 
 Definition Substn (ys:vars) (ds:dyns) (t:trm) : trm :=
   substn ys (encs ds) t.
@@ -419,8 +440,13 @@ Definition Substn (ys:vars) (ds:dyns) (t:trm) : trm :=
 (* ---------------------------------------------------------------------- *)
 (* ** Definition of lifted triples *)
 
+(** [Triple t H Q] describes a triple where the postcondition [Q] has
+    type [A->hprop] for some encodable type [A] *)
+
 Definition Triple (t:trm) `{EA:Enc A} (H:hprop) (Q:A->hprop) : Prop :=
   triple t H (Post Q).
+
+(** [Triple] satisfies [is_local], like [triple] does. *)
 
 Lemma is_local_Triple : forall t A `{EA:Enc A},
   is_local (@Triple t A EA).
@@ -443,6 +469,10 @@ Ltac xlocal_base tt ::=
 (* ---------------------------------------------------------------------- *)
 (* ** Lemma for changing the encoder in a triple *)
 
+(** [PostChange Q1 Q2] asserts that [Q1] of type [A1->hprop] entails
+    [Q2] of type [A2->hprop]. This predicate is used in the lemmas
+    that enable changing the type of the postcondition in a triple. *)
+
 Definition PostChange `{Enc A1} (Q1:A1->hprop) `{Enc A2} (Q2:A2->hprop) :=
   forall (X:A1), Q1 X ==> \exists (Y:A2), \[enc X = enc Y] \* Q2 Y.
 
@@ -456,11 +486,12 @@ Lemma Triple_enc_change :
   PostChange Q1 Q2 ->
   Triple t H Q2.
 Proof using.
-  introv M N. unfolds Triple. applys~ rule_conseq (rm M).
+  introv M N. unfolds Triple. applys~ triple_conseq (rm M).
   unfold Post. intros v. hpull ;=> V EV. subst. applys N.
 Qed.
 
-(** Specializations for converting from and to the raw values *)
+(** Specialization of [Triple_enc_change] for converting from a postcondition
+    of type [val->hprop]  *)
 
 Lemma Triple_enc_val_inv :
   forall (t:trm) (H:hprop) (Q1:val->hprop) `{EA2:Enc A2} (Q2:A2->hprop),
@@ -470,6 +501,9 @@ Lemma Triple_enc_val_inv :
 Proof using.
   introv M N. applys* (@Triple_enc_change val).
 Qed.
+
+(** Specialization of [Triple_enc_change] for converting to a postcondition
+    of type [val->hprop]  *)
 
 Lemma Triple_enc_val :
   forall A1 `{EA1:Enc A1} (t:trm) (H:hprop) (Q1:A1->hprop) (Q2:val->hprop),
@@ -488,210 +522,215 @@ Qed.
 (* ---------------------------------------------------------------------- *)
 (* ** Lifting of structural rules *)
 
-Lemma Rule_extract_hexists : forall t `{Enc A} B (J:B->hprop) (Q:A->hprop),
-  (forall x, Triple t (J x) Q) ->
-  Triple t (hexists J) Q.
-Proof using. intros. applys~ rule_extract_hexists. Qed.
-
-Lemma Rule_extract_hprop : forall t (P:Prop) `{Enc A} H (Q:A->hprop),
-  (P -> Triple t H Q) ->
-  Triple t (\[P] \* H) Q.
-Proof using. intros. applys~ rule_extract_hprop. Qed.
-
-Lemma Rule_consequence : forall t H' `{Enc A} (Q':A->hprop) H (Q:A->hprop),
+Lemma Triple_conseq : forall t H' `{Enc A} (Q':A->hprop) H (Q:A->hprop),
   H ==> H' ->
   Triple t H' Q' ->
   Q' ===> Q ->
   Triple t H Q.
-Proof using. introv MH M MQ. applys* rule_conseq MH. Qed.
+Proof using. introv MH M MQ. applys* triple_conseq MH. Qed.
 
-Lemma Rule_frame : forall t `{Enc A} H (Q:A->hprop) H',
+Lemma Triple_extract_hexists : forall t `{Enc A} B (J:B->hprop) (Q:A->hprop),
+  (forall x, Triple t (J x) Q) ->
+  Triple t (hexists J) Q.
+Proof using. intros. applys~ triple_extract_hexists. Qed.
+
+Lemma Triple_extract_hforall : forall t `{Enc A} B (J:B->hprop) (Q:A->hprop),
+  (exists x, Triple t (J x) Q) ->
+  Triple t (hforall J) Q.
+Proof using. intros. applys~ triple_extract_hforall. Qed.
+
+Lemma Triple_extract_hprop : forall t (P:Prop) `{Enc A} H (Q:A->hprop),
+  (P -> Triple t H Q) ->
+  Triple t (\[P] \* H) Q.
+Proof using. intros. applys~ triple_extract_hprop. Qed.
+
+Lemma Triple_extract_hwand_hpure_l : forall t (P:Prop) `{Enc A} H (Q:A->hprop),
+  P ->
+  Triple t H Q ->
+  Triple t (\[P] \-* H) Q.
+Proof using. intros. applys~ triple_extract_hwand_hpure_l. Qed.
+
+Lemma Triple_frame : forall t `{Enc A} H (Q:A->hprop) H',
   Triple t H Q ->
   Triple t (H \* H') (Q \*+ H').
 Proof using.
-  introv M. unfold Triple. rewrite Post_star. applys* rule_frame.
+  introv M. unfold Triple. rewrite Post_star. applys* triple_frame.
 Qed.
 
-Lemma Rule_htop_post : forall t H Q,
+Lemma Triple_htop_post : forall t `{Enc A} H (Q:A->hprop),
   Triple t H (Q \*+ \Top) ->
   Triple t H Q.
 Proof using.
-  introv M. unfolds Triple. rewrite Post_star in M. applys* rule_htop_post.
+  introv M. unfolds Triple. rewrite Post_star in M. applys* triple_htop_post.
 Qed.
 
-Lemma Rule_htop_pre : forall t H Q,
+Lemma Triple_htop_pre : forall t `{Enc A} H (Q:A->hprop),
   Triple t H Q ->
   Triple t (H \* \Top) Q.
-Proof using. introv M. applys* rule_htop_pre. Qed.
+Proof using. introv M. applys* triple_htop_pre. Qed.
+
+Lemma Triple_combined : forall t H1 H2 `{Enc A} (Q1 Q:A->hprop) H,
+  Triple t H1 Q1 ->
+  H ==> H1 \* H2 ->
+  Q1 \*+ H2 ===> Q \*+ \Top ->
+  Triple t H Q.
+Proof using.
+  introv M WH WQ. applys* triple_combined. 
+  do 2 rewrite <- Post_star. apply* Post_himpl.
+Qed.
 
 
 (* ---------------------------------------------------------------------- *)
 (* ** Lifting of term rules *)
 
-Lemma Rule_val : forall A `{EA:Enc A} (V:A) v H (Q:A->hprop),
+Lemma Triple_val : forall A `{EA:Enc A} (V:A) v H (Q:A->hprop),
   v = enc V ->
   H ==> Q V ->
   Triple (trm_val v) H Q.
 Proof using.
-  introv E M. applys rule_val. subst.
+  introv E M. applys triple_val. subst.
   unfold Post. hsimpl*.
 Qed.
 
-(* DEPRECATEd
-Lemma Rule_fun : forall x t1 H (Q:func->hprop),
-  H ==> Q (val_fun x t1) ->
-  Triple (trm_fun x t1) H Q.
-Proof using.
-  introv M. applys rule_fun. unfold Post. hsimpl*.
-Qed.
-*)
-
-Lemma Rule_fix : forall f x t1 H (Q:func->hprop),
+Lemma Triple_fix : forall f x t1 H (Q:func->hprop),
   H ==> Q (val_fix f x t1) ->
   Triple (trm_fix f x t1) H Q.
 Proof using.
-  introv M. applys rule_fix. unfold Post. hsimpl*.
+  introv M. applys triple_fix. unfold Post. hsimpl*.
 Qed.
 
-Lemma Rule_if : forall t0 t1 t2 H (Q1:bool->hprop) A `{EA:Enc A} (Q:A->hprop),
-  Triple t0 H Q1 ->
-  (forall (b:bool), Triple (if b then t1 else t2) (Q1 b) Q) ->
-  Triple (trm_if t0 t1 t2) H Q.
+Lemma Triple_let : forall z t1 t2 H,
+  forall A `{EA:Enc A} (Q:A->hprop) A1 `{EA1:Enc A1} (Q1:A1->hprop),
+  Triple t1 H Q1 ->
+  (forall (X:A1), Triple (Subst1 z X t2) (Q1 X) Q) ->
+  Triple (trm_let z t1 t2) H Q.
 Proof using.
-  introv M1 M2. applys* rule_if.
-  { intros b. unfold Post. xpull ;=> V E.
-    asserts E': (V = b). { destruct* V. } clears E. subst V. applys M2. }
-  { intros v N. unfold Post. hpull ;=> V E. subst. false N.
-    rewrite enc_bool_eq. hnfs*. } (* todo : simplify ?*)
+  introv M1 M2. applys triple_let M1. intros v. unfold Post at 1.
+  xpull. intros V E. subst. applys M2.
 Qed.
 
-Lemma Rule_seq : forall t1 t2 H,
+Lemma Triple_seq : forall t1 t2 H,
   forall A `{EA:Enc A} (Q:A->hprop) (Q1:unit->hprop),
   Triple t1 H Q1 ->
   Triple t2 (Q1 tt) Q ->
   Triple (trm_seq t1 t2) H Q.
 Proof using.
-  introv M1 M2. applys rule_seq.
+  introv M1 M2. applys triple_seq.
   { applys M1. }
   { intros X. unfold Post. xpull ;=> V E.
     destruct V. applys M2. }
 Qed.
 
-Lemma Rule_let : forall x t1 t2 H,
-  forall A `{EA:Enc A} (Q:A->hprop) A1 `{EA1:Enc A1} (Q1:A1->hprop),
-  Triple t1 H Q1 ->
-  (forall (X:A1), Triple (Subst1 x (Dyn X) t2) (Q1 X) Q) ->
-  Triple (trm_let x t1 t2) H Q.
+Lemma Triple_if : forall t0 t1 t2 H (Q1:bool->hprop) A `{EA:Enc A} (Q:A->hprop),
+  Triple t0 H Q1 ->
+  (forall (b:bool), Triple (if b then t1 else t2) (Q1 b) Q) ->
+  Triple (trm_if t0 t1 t2) H Q.
 Proof using.
-  introv M1 M2. applys rule_let M1. intros v. unfold Post at 1.
-  xpull. intros V E. subst. applys M2.
+  introv M1 M2. applys* triple_if.
+  { intros b. unfold Post. xpull ;=> V E.
+    asserts E': (V = b). { destruct* V. } clears E. subst V. applys M2. }
+  { intros v N. unfold Post. hpull ;=> V E. subst. false N.
+    rewrite enc_bool_eq. hnfs*. } (* LATER : simplify? *)
 Qed.
 
-(* TODO: investigate definition of (Subst A EA x (X:A) t2) *)
-
-Lemma Rule_apps_funs : forall xs F (Vs:dyns) t1 H A `{EA: Enc A} (Q:A->hprop),
+Lemma Triple_apps_funs : forall xs F (Vs:dyns) t1 H A `{EA: Enc A} (Q:A->hprop),
   F = (val_funs xs t1) ->
   var_funs (length Vs) xs ->
   Triple (Substn xs Vs t1) H Q ->
   Triple (trm_apps F (encs Vs)) H Q.
 Proof using.
-  introv E N M. unfold Triple. applys* rule_apps_funs. rewrite~ length_encs.
+  introv E N M. unfold Triple. applys* triple_apps_funs. rewrite~ length_encs.
 Qed.
 
-Lemma Rule_apps_fixs : forall xs (f:var) F (Vs:dyns) t1 H A `{EA: Enc A} (Q:A->hprop),
+Lemma Triple_apps_fixs : forall xs (f:var) F (Vs:dyns) t1 H A `{EA: Enc A} (Q:A->hprop),
   F = (val_fixs f xs t1) ->
   var_fixs f (length Vs) xs ->
   Triple (Substn (f::xs) ((Dyn F)::Vs) t1) H Q ->
   Triple (trm_apps F (encs Vs)) H Q.
 Proof using.
-  introv E N M. unfold Triple. applys* rule_apps_fixs. rewrite~ length_encs.
+  introv E N M. unfold Triple. applys* triple_apps_fixs. rewrite~ length_encs.
 Qed.
 
-
-(* ---------------------------------------------------------------------- *)
-(* ** Rules for loops *)
-
-Lemma Rule_while_raw : forall t1 t2 H A `{EA: Enc A} (Q:A->hprop),
+Lemma Triple_while_raw : forall t1 t2 H A `{EA: Enc A} (Q:A->hprop),
   Triple (trm_if t1 (trm_seq t2 (trm_while t1 t2)) val_unit) H Q ->
   Triple (trm_while t1 t2) H Q.
-Proof using. introv M. applys rule_while_raw. applys M. Qed.
+Proof using. introv M. applys triple_while_raw. applys M. Qed.
 
-Lemma Rule_for_raw : forall (x:var) (n1 n2:int) t3 H A `{EA: Enc A} (Q:A->hprop),
+Lemma Triple_for_raw : forall (x:var) (n1 n2:int) t3 H A `{EA: Enc A} (Q:A->hprop),
   Triple (
     If (n1 <= n2)
-      then (trm_seq (subst1 x n1 t3) (trm_for x (n1+1) n2 t3))
+      then (trm_seq (Subst1 x n1 t3) (trm_for x (n1+1) n2 t3))
       else val_unit) H Q ->
   Triple (trm_for x n1 n2 t3) H Q.
-Proof using. introv M. applys rule_for_raw. applys M. Qed.
-(* TODO: Should it be Subst1 above? *)
+Proof using. introv M. applys triple_for_raw. applys M. Qed.
 
 
 (* ---------------------------------------------------------------------- *)
-(** Primitive functions *)
-
-Implicit Types v : val.
-Implicit Types n : int.
-Implicit Types b : bool.
+(** Lifting of specitification of primitive functions *)
 
 Section RulesStateOps.
 Transparent Hsingle.
 
-Lemma Rule_ref : forall A `{EA:Enc A} (V:A),
+Lemma Triple_ref : forall A `{EA:Enc A} (V:A),
   Triple (val_ref ``V)
     \[]
     (fun l => l ~~> V).
-Proof using. intros. applys_eq rule_ref 1. subst~. Qed.
+Proof using. intros. applys_eq triple_ref 1. subst~. Qed.
 
-Lemma Rule_get : forall A `{EA:Enc A} (V:A) l,
+Lemma Triple_get : forall A `{EA:Enc A} (V:A) l,
   Triple (val_get ``l)
     (l ~~> V)
     (fun x => \[x = V] \* (l ~~> V)).
 Proof using.
-  introv. unfold Triple, Post. rewrite Hsingle_to_hsingle. xapplys* rule_get.
+  introv. unfold Triple, Post. rewrite Hsingle_to_hsingle. xapplys* triple_get.
 Qed.
 
-Lemma Rule_set' : forall v1 A2 `{EA2:Enc A2} (V2:A2) l,
+(** Specification of [set] allowing for change in type (i.e. strong update). *)
+
+Lemma Triple_set' : forall v1 A2 `{EA2:Enc A2} (V2:A2) l,
   Triple (val_set ``l ``V2)
     (l ~~> v1)
     (fun u => l ~~> V2).
 Proof using.
-  intros. unfold Triple. rewrite Hsingle_to_hsingle. xapplys rule_set.
+  intros. unfold Triple. rewrite Hsingle_to_hsingle. xapplys triple_set.
   intros. subst. unfold Post. hsimpl~ tt.
 Qed.
 
-Lemma Rule_set : forall A1 A2 `{EA1:Enc A1} (V1:A1) `{EA2:Enc A2} (V2:A2) l,
+(** Specification of [set] for writes preserving the type. *)
+
+Lemma Triple_set : forall A1 A2 `{EA1:Enc A1} (V1:A1) `{EA2:Enc A2} (V2:A2) l,
   Triple (val_set l ``V2)
     (l ~~> V1)
     (fun u => l ~~> V2).
-Proof using. intros. applys~ Rule_set'. Qed.
+Proof using. intros. applys~ Triple_set'. Qed.
 
-End RulesStateOps.
-
-Lemma Rule_alloc : forall n,
+Lemma Triple_alloc : forall n,
   n >= 0 ->
   Triple (val_alloc n)
     \[]
     (fun l => \[l <> null] \* Alloc (abs n) l).
 Proof using.
-  introv N. unfold Triple, Post. xapplys* rule_alloc.
+  introv N. unfold Triple, Post. xapplys* triple_alloc.
 Qed.
 
-Lemma Rule_alloc_nat : forall (n:nat),
-  Triple (val_alloc (n:int))
+Lemma Triple_alloc_nat : forall (k:nat),
+  Triple (val_alloc (k:int))
     \[]
-    (fun l => \[l <> null] \* Alloc n l).
+    (fun l => \[l <> null] \* Alloc k l).
 Proof using.
-  intros. xapplys~ Rule_alloc. { math. }
+  intros. xapplys~ Triple_alloc. { math. }
   { intros. rewrite abs_nat. hsimpl. }
 Qed.
 
-Lemma Rule_eq_val : forall v1 v2,
+End RulesStateOps.
+
+Lemma Triple_eq_val : forall v1 v2,
   Triple (val_eq v1 v2)
     \[]
     (fun b => \[ b = isTrue (v1 = v2) ]).
-Proof using. intros. unfold Triple, Post. xapplys~ rule_eq. Qed.
+Proof using. intros. unfold Triple, Post. xapplys~ triple_eq. Qed.
 
-Lemma Rule_eq : forall `{EA:Enc A},
+Lemma Triple_eq : forall `{EA:Enc A},
   Enc_injective EA ->
   forall (v1 v2 : A),
   Triple (val_eq ``v1 ``v2)
@@ -699,203 +738,32 @@ Lemma Rule_eq : forall `{EA:Enc A},
     (fun (b:bool) => \[b = isTrue (v1 = v2)]).
 Proof using.
   introv I. intros.
-  applys (@Triple_enc_change bool). { sapply Rule_eq_val. } (* todo: why sapply ? *)
+  applys (@Triple_enc_change bool). { sapply Triple_eq_val. } (* todo: why sapply ? *)
   unfolds. hpulls. hsimpl*. unfolds Enc_injective. unfolds injective.
   rewrite~ Enc_injective_eq.
 Qed.
 
-Lemma Rule_add : forall n1 n2,
+Lemma Triple_add : forall n1 n2,
   Triple (val_add n1 n2)
     \[]
     (fun n => \[n = n1 + n2]).
-Proof using. intros. unfold Triple, Post. xapplys~ rule_add. Qed.
+Proof using. intros. unfold Triple, Post. xapplys~ triple_add. Qed.
 
-Lemma Rule_sub : forall n1 n2,
+Lemma Triple_sub : forall n1 n2,
   Triple (val_sub n1 n2)
     \[]
     (fun n => \[n = n1 - n2]).
-Proof using. intros. unfold Triple, Post. xapplys~ rule_sub. Qed.
+Proof using. intros. unfold Triple, Post. xapplys~ triple_sub. Qed.
 
-(* TODO: add other arithmetic primitives *)
-
-Lemma Rule_ptr_add : forall (l:loc) (n:int),
+Lemma Triple_ptr_add : forall (l:loc) (n:int),
   (l:nat) + n >= 0 ->
   Triple (val_ptr_add l n)
     \[]
     (fun l' => \[(l':nat) = abs ((l:nat) + n)]).
-Proof using. intros. unfold Triple, Post. xapplys~ rule_ptr_add. Qed.
+Proof using. intros. unfold Triple, Post. xapplys~ triple_ptr_add. Qed.
 
-Lemma Rule_ptr_add_nat : forall (l:loc) (f:nat),
+Lemma Triple_ptr_add_nat : forall (l:loc) (f:nat),
   Triple (val_ptr_add l f)
     \[]
     (fun l' => \[(l':nat) = (l+f)%nat]).
-Proof using. intros. unfold Triple, Post. xapplys~ rule_ptr_add_nat. Qed.
-
-
-
-(* ********************************************************************** *)
-(* * Bonus *)
-
-(* DEPRECATED?
-
-(* ---------------------------------------------------------------------- *)
-(** Reformulation of rule for N-ary functions *)
-
-Definition Spec_funs (xs:vars) (t1:trm) (F:val) :=
-  forall (Xs:dyns), length xs = length Xs ->
-    Triple (Substn xs Xs t1) ===> Triple (trm_apps F (encs Xs)).
-
-Lemma spec_funs_val_funs : forall xs t1,
-  var_distinct xs ->
-  xs <> nil ->
-  Spec_funs xs t1 (val_funs xs t1).
-Proof using. introv D N E M. applys* Rule_apps_funs. splits~. Qed.
-
-
-(* ---------------------------------------------------------------------- *)
-(** Reformulation of rule for N-ary recursive functions *)
-
-Definition Spec_fixs (f:var) (xs:vars) (t1:trm) (F:val) :=
-  forall (Xs:dyns), length xs = length Xs ->
-    Triple (subst1 f F (Substn xs Xs t1)) ===> Triple (trm_apps F (encs Xs)).
-
-Lemma Spec_fixs_val_fixs : forall f xs t1,
-  var_distinct (f::xs) ->
-  xs <> nil ->
-  Spec_fixs f xs t1 (val_fixs f xs t1).
-Proof using. introv D N L M. applys* Rule_apps_fixs. splits~. Qed.
-
-
-(* ---------------------------------------------------------------------- *)
-(** Functions of one argument *)
-
-(* TODO: upper case arguments that are encoded *)
-
-Lemma Rule_app_fun : forall x F V t1 H A `{EA: Enc A} (Q:A->hprop),
-  F = (val_fun x t1) ->
-  Triple (subst x V t1) H Q ->
-  Triple (trm_app F V) H Q.
-Proof using. introv EF M. applys* rule_app_fun. Qed.
-
-Definition Spec_fun (x:var) (t1:trm) (F:val) :=
-  forall X, Triple (subst x X t1) ===> Triple (trm_app F X).
-
-Lemma Spec_fun_val_fun : forall x t1,
-  Spec_fun x t1 (val_fun x t1).
-Proof using. introv. intros X H Q M. applys* Rule_app_fun. Qed.
-
-Lemma Rule_fun_spec : forall x t1 H (Q:func->hprop),
-  (forall (F:val), Spec_fun x t1 F -> H ==> Q F) ->
-  Triple (trm_fun x t1) H Q.
-Proof using.
-  introv M. forwards M': (rm M) (val_fun x t1).
-  { applys Spec_fun_val_fun. }
-  { applys~ Rule_fun. }
-Qed.
-
-Lemma Rule_let_fun : forall f x t1 t2 H A `{EA: Enc A} (Q:A->hprop),
-  (forall (F:val), Spec_fun x t1 F -> Triple (subst f F t2) H Q) ->
-  Triple (trm_let f (trm_fun x t1) t2) H Q.
-Proof using.
-  introv M. applys Rule_let (fun F => \[Spec_fun x t1 F] \* H).
-  { applys Rule_fun_spec. introv HF. hsimpl~. }
-  { intros F. applys Rule_extract_hprop. applys M. }
-Qed.
-
-(* ---------------------------------------------------------------------- *)
-(** Recursive functions of one argument *)
-
-Lemma Rule_app_fix : forall f x F V t1 H A `{EA: Enc A} (Q:A->hprop),
-  F = (val_fix f x t1) ->
-  Triple (subst f F (subst x V t1)) H Q ->
-  Triple (trm_app F V) H Q.
-Proof using. introv EF M. applys* rule_app_fix. Qed.
-
-Definition Spec_fix (f:var) (x:var) (t1:trm) (F:val) :=
-  forall X, Triple (subst f F (subst x X t1)) ===> Triple (trm_app F X).
-
-Lemma Spec_fix_val_fix : forall f x t1,
-  Spec_fix f x t1 (val_fix f x t1).
-Proof using. introv. intros X H Q M. applys* Rule_app_fix. Qed.
-
-Lemma Rule_fix_spec : forall f x t1 H (Q:func->hprop),
-  (forall (F:val), Spec_fix f x t1 F -> H ==> Q F) ->
-  Triple (trm_fix f x t1) H Q.
-Proof using.
-  introv M. forwards M': (rm M) (val_fix f x t1).
-  { applys Spec_fix_val_fix. }
-  { applys~ Rule_fix. }
-Qed.
-
-Lemma Rule_let_fix : forall f x t1 t2 H A `{EA: Enc A} (Q:A->hprop),
-  (forall (F:val), Spec_fix f x t1 F -> Triple (subst f F t2) H Q) ->
-  Triple (trm_let f (trm_fix f x t1) t2) H Q.
-Proof using.
-  introv M. applys Rule_let (fun F => \[Spec_fix f x t1 F] \* H).
-  { applys Rule_fix_spec. introv HF. hsimpl~. }
-  { intros F. applys Rule_extract_hprop. applys M. }
-Qed.
-
-
-(* ---------------------------------------------------------------------- *)
-(** Derived rules *)
-
-Lemma Rule_if' : forall t0 t1 t2 H (Q1:bool->hprop) A `{EA:Enc A} (Q:A->hprop),
-  Triple t0 H Q1 ->
-  Triple t1 (Q1 true) Q ->
-  Triple t2 (Q1 false) Q ->
-  Triple (trm_if t0 t1 t2) H Q.
-Proof using.
-  introv M0 M1 M2. applys* Rule_if. { intros b. case_if*. }
-Qed.
-
-Lemma Rule_let_val : forall A1 `{Enc A1} (V1:A1) x v1 t2 H A `{EA: Enc A} (Q:A->hprop),
-  v1 = enc V1 ->
-  (forall X, X = V1 -> Triple (Subst x (Dyn X) t2) H Q) ->
-  Triple (trm_let x (trm_val v1) t2) H Q.
-Proof using.
-  introv E M. applys rule_let_val. intros X EX. subst. applys~ M.
-Qed.
-
-*)
-
-(* ---------------------------------------------------------------------- *)
-(** Other rules for loops *)
-
-(*
-Lemma Rule_while : forall t1 t2 H Q,
-  (forall t,
-     (forall H' Q', triple (trm_if t1 (trm_seq t2 t) val_unit) H' Q' ->
-                    triple t H' Q') ->
-    triple t H Q) ->
-  triple (trm_while t1 t2) H Q.
-
-Lemma Rule_while_inv : forall (A:Type) (I:bool->A->hprop) (R:A->A->Prop) t1 t2 H,
-  let Q := (fun r => \exists Y, I false Y) in
-  wf R ->
-  (H ==> (\exists b X, I b X) \* \Top) ->
-  (forall t b X,
-      (forall b' X', R X' X -> triple t (I b' X') Q) ->
-      triple (trm_if t1 (trm_seq t2 t) val_unit) (I b X) Q) ->
-  triple (trm_while t1 t2) H Q.
-
-Lemma Rule_for_gt : forall x n1 n2 t3 H Q,
-  n1 > n2 ->
-  (fun r => \* H) ===> (Q \*+ \Top) ->
-  triple (trm_for x n1 n2 t3) H Q.
-
-Lemma Rule_for_le : forall Q1 x n1 n2 t3 H Q,
-  n1 <= n2 ->
-  triple (subst x n1 t3) H Q1 ->
-  triple (trm_for x (n1+1) n2 t3) (Q1 val_unit) Q ->
-  (forall v, ~ is_val_unit v -> (Q1 v) ==> \[False]) ->
-  triple (trm_for x n1 n2 t3) H Q.
-
-Lemma Rule_for_inv : forall (I:int->hprop) H' x n1 n2 t3 H Q,
-  (n1 <= n2+1) ->
-  (H ==> I n1 \* H') ->
-  (forall i, n1 <= i <= n2 ->
-     triple (subst x i t3) (I i) (fun r => I (i+1))) ->
-  (I (n2+1) \* H' ==> Q val_unit \* \Top) ->
-  triple (trm_for x n1 n2 t3) H Q.
-*)
+Proof using. intros. unfold Triple, Post. xapplys~ triple_ptr_add_nat. Qed.
