theories/ExampleList.v
@@ -215,13 +215,13 @@ Definition val_new_cell :=
     'p.
 *)
 
-Lemma Rule_new_cell : forall `{EA:Enc A} (x:A) (q:loc),
+Lemma Triple_new_cell : forall `{EA:Enc A} (x:A) (q:loc),
   Triple (val_new_cell ``x ``q)
     PRE \[]
     POST (fun p => (p ~> MCell x q)).
-Proof using. xrule_new_record. Qed.
+Proof using. xtriple_new_record. Qed.
 
-Hint Extern 1 (Register_Spec val_new_cell) => Provide Rule_new_cell.
+Hint Extern 1 (Register_Spec val_new_cell) => Provide Triple_new_cell.
 
 Opaque val_new_cell.
 
@@ -241,13 +241,13 @@ Definition val_is_empty :=
     Let 'y := val_get_tl 'p in
     val_eq 'x 'y.
 
-Parameter Rule_is_empty : forall `{EA:Enc A} (L:list A) p,
+Parameter Triple_is_empty : forall `{EA:Enc A} (L:list A) p,
   Triple (val_is_empty p)
     (p ~> MQueue L)
     (fun r => \[r = isTrue (L = nil)] \* p ~> MQueue L).
 (* LATER: similar proof to ExampleQueueNonLifted, todo *)
 
-Hint Extern 1 (Register_Spec val_is_empty) => Provide Rule_is_empty.
+Hint Extern 1 (Register_Spec val_is_empty) => Provide Triple_is_empty.
 
 Definition val_transfer :=
   ValFun 'p1 'p2 :=
@@ -264,7 +264,7 @@ Definition val_transfer :=
        val_set_tl 'p2 'f2
     End.
 
-Lemma Rule_transfer : forall `{EA:Enc A} (L1 L2:list A) p1 p2,
+Lemma Triple_transfer : forall `{EA:Enc A} (L1 L2:list A) p1 p2,
   Triple (val_transfer p1 p2)
     (p1 ~> MQueue L1 \* p2 ~> MQueue L2)
     (fun (_:unit) => p1 ~> MQueue (L1 ++ L2) \* p2 ~> MQueue nil).
@@ -295,7 +295,7 @@ Definition val_mlist_copy :=
       val_new_cell 'x 'p2
    ).
 
-Lemma Rule_mlist_copy : forall p (L:list int),
+Lemma Triple_mlist_copy : forall p (L:list int),
   Triple (val_mlist_copy ``p)
     PRE (p ~> MList L)
     POST (fun (p':loc) =>
@@ -309,7 +309,7 @@ Proof using.
     intros p'. do 2 rewrite MList_cons_eq. hsimpl. }
 Qed.
 
-Hint Extern 1 (Register_Spec val_mlist_copy) => Provide Rule_mlist_copy.
+Hint Extern 1 (Register_Spec val_mlist_copy) => Provide Triple_mlist_copy.
 
 
 
@@ -328,7 +328,7 @@ Definition val_mlist_length : val :=
       0
     ).
 
-Lemma Rule_mlist_length : forall A `{EA:Enc A} (L:list A) (p:loc),
+Lemma Triple_mlist_length : forall A `{EA:Enc A} (L:list A) (p:loc),
   Triple (val_mlist_length ``p)
     PRE (p ~> MList L)
     POST (fun (r:int) => \[r = length L] \* p ~> MList L).
@@ -356,7 +356,7 @@ Definition val_mlist_append : val :=
       val_new_cell 'x 'p
     ).
 
-Lemma Rule_mlist_append : forall (L1 L2:list int) (p1 p2:loc),
+Lemma Triple_mlist_append : forall (L1 L2:list int) (p1 p2:loc),
   Triple (val_mlist_append ``p1 ``p2)
     PRE (p1 ~> MList L1 \* p2 ~> MList L2)
     POST (fun (p:loc) =>
@@ -376,7 +376,7 @@ Qed.
 (* ********************************************************************** *)
 (* * Out-of-place append of two aliased mutable lists *)
 
-Lemma Rule_mlist_append_aliased : forall (L:list int) (p1:loc),
+Lemma Triple_mlist_append_aliased : forall (L:list int) (p1:loc),
   Triple (val_mlist_append ``p1 ``p1)
     PRE (p1 ~> MList L)
     POST (fun (p:loc) => p ~> MList (L++L) \* p1 ~> MList L).
@@ -415,7 +415,7 @@ Definition val_mlist_iter : val :=
       'g 'f 'q
     End.
 
-Lemma Rule_mlist_iter : forall `{EA:Enc A} (I:list A->hprop) (L:list A) (f:func) (p:loc),
+Lemma Triple_mlist_iter : forall `{EA:Enc A} (I:list A->hprop) (L:list A) (f:func) (p:loc),
   (forall x K,
     Triple (f ``x)
       PRE (I K)
@@ -441,7 +441,7 @@ Proof using.
     xvals~. }
 Qed.
 
-Lemma Rule_mlist_iter_general : forall `{EA:Enc A} (I:list A->hprop) (L:list A) (f:func) (p:loc),
+Lemma Triple_mlist_iter_general : forall `{EA:Enc A} (I:list A->hprop) (L:list A) (f:func) (p:loc),
   (forall x L1 L2, L = L1++x::L2 ->
     Triple (f ``x)
       PRE (I L1)
@@ -478,13 +478,13 @@ Definition val_mlist_length_using_iter : val :=
     val_mlist_iter 'f 'p ;;;
     val_get 'r.
 
-Lemma Rule_mlist_length_using_iter : forall A `{EA:Enc A} (L:list A) (p:loc),
+Lemma Triple_mlist_length_using_iter : forall A `{EA:Enc A} (L:list A) (p:loc),
   Triple (val_mlist_length_using_iter ``p)
     PRE (p ~> MList L)
     POST (fun (r:int) => \[r = length L] \* p ~> MList L).
 Proof using.
   xcf. xapps ;=> R. xval ;=> F HF.
-  xapp (@Rule_mlist_iter _ _ (fun (K:list A) => R ~~> length K)).
+  xapp (@Triple_mlist_iter _ _ (fun (K:list A) => R ~~> length K)).
   { intros x K. xcf. unfold Substn, substn; simpl. (* todo: Unfold *)
     xapp. hsimpl. rew_list; math. }
   xapps ;=> r Hr. hsimpl~.
@@ -509,7 +509,7 @@ Definition val_mlist_length_loop : val :=
     Done ;;;
     val_get 'n.
 
-Lemma Rule_mlist_length_loop : forall A `{EA:Enc A} (L:list A) (p:loc),
+Lemma Triple_mlist_length_loop : forall A `{EA:Enc A} (L:list A) (p:loc),
   Triple (val_mlist_length_loop ``p)
     PRE (p ~> MList L)
     POST (fun (r:int) => \[r = length L] \* p ~> MList L).
@@ -550,7 +550,7 @@ Definition val_mlist_incr : val :=
       'f 'q
     ) End.
 
-Lemma Rule_mlist_incr : forall (L:list int) (p:loc),
+Lemma Triple_mlist_incr : forall (L:list int) (p:loc),
   Triple (val_mlist_incr ``p)
     PRE (p ~> MList L)
     POST (fun (r:unit) => p ~> MList (LibList.map (fun x => x+1) L)).
@@ -582,7 +582,7 @@ Definition val_mlist_in_place_rev : val :=
     Done ;;;
     val_get 's.
 
-Lemma Rule_mlist_in_place_rev : forall A `{EA:Enc A} (L:list A) (p:loc),
+Lemma Triple_mlist_in_place_rev : forall A `{EA:Enc A} (L:list A) (p:loc),
   Triple (val_mlist_in_place_rev ``p)
     PRE (p ~> MList L)
     POST (fun (p':loc) => p' ~> MList (rev L)).
@@ -622,7 +622,7 @@ Definition val_mlist_cps_append : val :=
       'f 't 'q 'k2
     ).
 
-Lemma Rule_mlist_cps_append : forall A `{EA:Enc A} (L M:list A) (p q:loc) (k:func),
+Lemma Triple_mlist_cps_append : forall A `{EA:Enc A} (L M:list A) (p q:loc) (k:func),
   forall `{EB: Enc B} (H:hprop) (Q:B->hprop),
   (forall (r:loc), Triple (k ``r)
      PRE (r ~> MList (L ++ M) \* H)
