theories/LambdaSepCredits.v
@@ -563,7 +563,7 @@ Definition pay_one H H' :=
 (* ---------------------------------------------------------------------- *)
 (* ** Structural rules *)
 
-Lemma rule_extract_hexists : forall t (A:Type) (J:A->hprop) Q,
+Lemma triple_extract_hexists : forall t (A:Type) (J:A->hprop) Q,
   (forall x, triple t (J x) Q) ->
   triple t (hexists J) Q.
 Proof using.
@@ -571,15 +571,15 @@ Proof using.
   destruct N as (x&N). applys* M.
 Qed.
 
-Lemma rule_extract_hprop : forall t (P:Prop) H Q,
+Lemma triple_extract_hprop : forall t (P:Prop) H Q,
   (P -> triple t H Q) ->
   triple t (\[P] \* H) Q.
 Proof using.
-  intros t. applys (rule_extract_hprop_from_extract_hexists (triple t)).
-  applys rule_extract_hexists.
+  intros t. applys (triple_extract_hprop_from_extract_hexists (triple t)).
+  applys triple_extract_hexists.
 Qed.
 
-Lemma rule_conseq : forall t H' Q' H Q,
+Lemma triple_conseq : forall t H' Q' H Q,
   H ==> H' ->
   triple t H' Q' ->
   Q' ===> Q ->
@@ -590,7 +590,7 @@ Proof using.
   exists n h' v. splits~. { hhsimpl. hchanges~ (MQ v). }
 Qed.
 
-Lemma rule_frame : forall t H Q H',
+Lemma triple_frame : forall t H Q H',
   triple t H Q ->
   triple t (H \* H') (Q \*+ H').
 Proof using.
@@ -599,7 +599,7 @@ Proof using.
   exists n h' v. splits~. { hhsimpl~. }
 Qed.
 
-Lemma rule_htop_post : forall t H Q,
+Lemma triple_htop_post : forall t H Q,
   triple t H (Q \*+ \Top) ->
   triple t H Q.
 Proof using.
@@ -607,18 +607,18 @@ Proof using.
   exists n h' v. splits~. { rewrite <- htop_hstar_htop. hhsimpl. }
 Qed.
 
-Lemma rule_htop_pre : forall t H Q,
+Lemma triple_htop_pre : forall t H Q,
   triple t H Q ->
   triple t (H \* \Top) Q.
 Proof using.
-  introv M. applys rule_htop_post. applys~ rule_frame.
+  introv M. applys triple_htop_post. applys~ triple_frame.
 Qed.
 
 
 (* ---------------------------------------------------------------------- *)
 (* ** Term rules *)
 
-Lemma rule_val : forall v H Q,
+Lemma triple_val : forall v H Q,
   H ==> Q v ->
   triple (trm_val v) H Q.
 Proof using.
@@ -627,7 +627,7 @@ Proof using.
   { hhsimpl. hchanges M. }
 Qed.
 
-Lemma rule_fix : forall (f z:bind) t1 H Q,
+Lemma triple_fix : forall (f z:bind) t1 H Q,
   H ==> Q (val_fix f z t1) ->
   triple (trm_fix f z t1) H Q.
 Proof using.
@@ -640,7 +640,7 @@ Qed.
 Definition is_val_bool (v:val) : Prop :=
   exists b, v = val_bool b.
 
-Lemma rule_if : forall Q1 t0 t1 t2 H Q,
+Lemma triple_if : forall Q1 t0 t1 t2 H Q,
   triple t0 H Q1 ->
   (forall (b:bool), triple (if b then t1 else t2) (Q1 b) Q) ->
   (forall v, ~ is_val_bool v -> (Q1 v) ==> \[False]) ->
@@ -661,18 +661,18 @@ Proof using.
     lets: hpure_inv Z. false*. } (* TODO: shorten this *)
 Qed.
 
-Lemma rule_if_bool : forall (b:bool) t1 t2 H Q,
+Lemma triple_if_bool : forall (b:bool) t1 t2 H Q,
   (b = true -> triple t1 H Q) ->
   (b = false -> triple t2 H Q) ->
   triple (trm_if b t1 t2) H Q.
 Proof using.
-  introv M1 M2. applys rule_if (fun r => \[r = val_bool b] \* H).
-  { applys rule_val. hsimpl~. }
-  { intros b'. applys~ rule_extract_hprop. intros E. inverts E. case_if*. }
+  introv M1 M2. applys triple_if (fun r => \[r = val_bool b] \* H).
+  { applys triple_val. hsimpl~. }
+  { intros b'. applys~ triple_extract_hprop. intros E. inverts E. case_if*. }
   { intros v' N. hpull. intros E. inverts~ E. false N. hnfs*. }
 Qed.
 
-Lemma rule_let : forall z t1 t2 H Q Q1,
+Lemma triple_let : forall z t1 t2 H Q Q1,
   triple t1 H Q1 ->
   (forall (X:val), triple (subst1 z X t2) (Q1 X) Q) ->
   triple (trm_let z t1 t2) H Q.
@@ -686,17 +686,17 @@ Proof using.
   { math. }
 Qed.
 
-Lemma rule_let_val : forall z v1 t2 H Q,
+Lemma triple_let_val : forall z v1 t2 H Q,
   (forall (X:val), X = v1 -> triple (subst1 z X t2) H Q) ->
   triple (trm_let z (trm_val v1) t2) H Q.
 Proof using.
   introv M. forwards~ M': (rm M).
-  applys_eq~ (>> rule_let H (fun x => \[x = v1] \* H)) 2.
-  { applys rule_val. hsimpl~. }
-  { intros X. applys rule_extract_hprop. intro_subst. applys M'. }
+  applys_eq~ (>> triple_let H (fun x => \[x = v1] \* H)) 2.
+  { applys triple_val. hsimpl~. }
+  { intros X. applys triple_extract_hprop. intro_subst. applys M'. }
 Qed.
 
-Lemma rule_app_fix : forall f x F V t1 H H' Q,
+Lemma triple_app_fix : forall f x F V t1 H H' Q,
   F = (val_fix f x t1) ->
   pay_one H H' ->
   triple (subst2 f F x V t1) H' Q ->
@@ -717,7 +717,7 @@ Qed.
 Section RulesPrimitiveOps.
 Transparent hstar hsingle.
 
-Lemma rule_ref : forall v,
+Lemma triple_ref : forall v,
   triple (val_ref v)
     \[]
     (fun r => \exists l, \[r = val_loc l] \* l ~~~> v).
@@ -732,7 +732,7 @@ Proof using.
     { splits~. hhsimpl~. } }
 Qed.
 
-Lemma rule_get : forall v l,
+Lemma triple_get : forall v l,
   triple (val_get (val_loc l))
     (l ~~~> v)
     (fun x => \[x = v] \* (l ~~~> v)).
@@ -745,7 +745,7 @@ Proof using.
   { rew_heap. rewrite hstar_pure. split~. hhsimpl~. }
 Qed.
 
-Lemma rule_set : forall w l v,
+Lemma triple_set : forall w l v,
   triple (val_set (val_loc l) w)
     (l ~~~> v)
     (fun r => \[r = val_unit] \* l ~~~> w).
@@ -876,12 +876,12 @@ Definition spec_fix (f:var) (x:var) (t1:trm) (F:val) :=
     triple (subst2 f F x X t1) H' Q ->
     triple (trm_app F X) H Q.
 
-Lemma rule_let_fix : forall f x t1 t2 H Q,
+Lemma triple_let_fix : forall f x t1 t2 H Q,
   (forall (F:val), spec_fix f x t1 F -> triple (subst1 f F t2) H Q) ->
   triple (trm_let f (trm_fix f x t1) t2) H Q.
 Proof using.
-  introv M. applys rule_let (fun F => \[spec_fix f x t1 F] \* H).
-  { applys rule_fix. hsimpl~.
-    intros F H' H'' Q' M1 M2. applys* rule_app_fix. }
-  { intros F. applys rule_extract_hprop. applys M. }
+  introv M. applys triple_let (fun F => \[spec_fix f x t1 F] \* H).
+  { applys triple_fix. hsimpl~.
+    intros F H' H'' Q' M1 M2. applys* triple_app_fix. }
+  { intros F. applys triple_extract_hprop. applys M. }
 Qed.
