theories/LambdaSepLowLevel.v
@@ -67,7 +67,7 @@ Ltac xlocal_base tt ::=
 (** Note: all these rules could be derived directly from the fact that
     [triple] satisfies [is_local], using lemmas from [SepFunctor] *)
 
-Lemma rule_extract_hexists : forall t (A:Type) (J:A->hprop) Q,
+Lemma triple_extract_hexists : forall t (A:Type) (J:A->hprop) Q,
   (forall x, triple t (J x) Q) ->
   triple t (hexists J) Q.
 Proof using.
@@ -75,7 +75,7 @@ Proof using.
   destruct N as (x&N). applys* M.
 Qed.
 
-Lemma rule_extract_hforall : forall t (A:Type) (J:A->hprop) Q,
+Lemma triple_extract_hforall : forall t (A:Type) (J:A->hprop) Q,
   (exists x, triple t (J x) Q) ->
   triple t (hforall J) Q.
 Proof using.
@@ -83,15 +83,15 @@ Proof using.
   applys* M.
 Qed.
 
-Lemma rule_extract_hprop : forall t (P:Prop) H Q,
+Lemma triple_extract_hprop : forall t (P:Prop) H Q,
   (P -> triple t H Q) ->
   triple t (\[P] \* H) Q.
 Proof using.
-  intros t. applys (rule_extract_hprop_from_extract_hexists (triple t)).
-  applys rule_extract_hexists.
+  intros t. applys (triple_extract_hprop_from_extract_hexists (triple t)).
+  applys triple_extract_hexists.
 Qed.
 
-Lemma rule_extract_hwand_hpure_l : forall t (P:Prop) H Q,
+Lemma triple_extract_hwand_hpure_l : forall t (P:Prop) H Q,
   P ->
   triple t H Q ->
   triple t (\[P] \-* H) Q.
@@ -103,7 +103,7 @@ Proof using.
   applys* M.
 Qed.
 
-Lemma rule_conseq : forall t H' Q' H Q,
+Lemma triple_conseq : forall t H' Q' H Q,
   H ==> H' ->
   triple t H' Q' ->
   Q' ===> Q ->
@@ -114,7 +114,7 @@ Proof using.
   exists h' v. splits~. { hhsimpl. hchanges (MQ v). }
 Qed.
 
-Lemma rule_frame : forall t H Q H',
+Lemma triple_frame : forall t H Q H',
   triple t H Q ->
   triple t (H \* H') (Q \*+ H').
 Proof using.
@@ -123,7 +123,7 @@ Proof using.
   exists h' v. splits~. { hhsimpl~. }
 Qed.
 
-Lemma rule_htop_post : forall t H Q,
+Lemma triple_htop_post : forall t H Q,
   triple t H (Q \*+ \Top) ->
   triple t H Q.
 Proof using.
@@ -131,18 +131,18 @@ Proof using.
   exists h' v. splits~. { rewrite <- htop_hstar_htop. hhsimpl. }
 Qed.
 
-Lemma rule_htop_pre : forall t H Q,
+Lemma triple_htop_pre : forall t H Q,
   triple t H Q ->
   triple t (H \* \Top) Q.
 Proof using.
-  introv M. applys rule_htop_post. applys~ rule_frame.
+  introv M. applys triple_htop_post. applys~ triple_frame.
 Qed.
 
 
 (* ---------------------------------------------------------------------- *)
 (* ** Term rules *)
 
-Lemma rule_val : forall v H Q,
+Lemma triple_val : forall v H Q,
   H ==> Q v ->
   triple (trm_val v) H Q.
 Proof using.
@@ -152,7 +152,7 @@ Proof using.
 Qed.
 
 (*
-Lemma rule_fun : forall x t1 H Q,
+Lemma triple_fun : forall x t1 H Q,
   H ==> Q (val_fun x t1) ->
   triple (trm_fun x t1) H Q.
 Proof using.
@@ -162,7 +162,7 @@ Proof using.
 Qed.
 *)
 
-Lemma rule_fix : forall (f z:bind) t1 H Q,
+Lemma triple_fix : forall (f z:bind) t1 H Q,
   H ==> Q (val_fix f z t1) ->
   triple (trm_fix f z t1) H Q.
 Proof using.
@@ -171,7 +171,7 @@ Proof using.
   { hhsimpl. hchanges M. }
 Qed.
 
-Lemma rule_if : forall Q1 t0 t1 t2 H Q,
+Lemma triple_if : forall Q1 t0 t1 t2 H Q,
   triple t0 H Q1 ->
   (forall (b:bool), triple (if b then t1 else t2) (Q1 b) Q) ->
   (forall v, ~ is_val_bool v -> (Q1 v) ==> \[False]) ->
@@ -191,18 +191,18 @@ Proof using.
     lets: hpure_inv Z. false*. } (* LATER: shorten this *)
 Qed.
 
-Lemma rule_if_bool : forall (b:bool) t1 t2 H Q,
+Lemma triple_if_bool : forall (b:bool) t1 t2 H Q,
   (b = true -> triple t1 H Q) ->
   (b = false -> triple t2 H Q) ->
   triple (trm_if b t1 t2) H Q.
 Proof using.
-  introv M1 M2. applys rule_if (fun r => \[r = val_bool b] \* H).
-  { applys rule_val. hsimpl~. }
-  { intros b'. applys~ rule_extract_hprop. intros E. inverts E. case_if*. }
+  introv M1 M2. applys triple_if (fun r => \[r = val_bool b] \* H).
+  { applys triple_val. hsimpl~. }
+  { intros b'. applys~ triple_extract_hprop. intros E. inverts E. case_if*. }
   { intros v' N. hpull. intros E. inverts~ E. false N. hnfs*. }
 Qed.
 
-Lemma rule_seq : forall t1 t2 H Q Q1,
+Lemma triple_seq : forall t1 t2 H Q Q1,
   triple t1 H Q1 ->
   (forall (X:val), triple t2 (Q1 X) Q) ->
   triple (trm_seq t1 t2) H Q.
@@ -215,7 +215,7 @@ Proof using.
   { rewrite <- htop_hstar_htop. hhsimpl. }
 Qed.
 
-Lemma rule_let : forall z t1 t2 H Q Q1,
+Lemma triple_let : forall z t1 t2 H Q Q1,
   triple t1 H Q1 ->
   (forall (X:val), triple (subst1 z X t2) (Q1 X) Q) ->
   triple (trm_let z t1 t2) H Q.
@@ -228,7 +228,7 @@ Proof using.
   { rewrite <- htop_hstar_htop. hhsimpl. }
 Qed.
 
-Lemma rule_apps_funs : forall xs F (Vs:vals) t1 H Q,
+Lemma triple_apps_funs : forall xs F (Vs:vals) t1 H Q,
   F = (val_funs xs t1) ->
   var_funs (length Vs) xs ->
   triple (substn xs Vs t1) H Q ->
@@ -238,7 +238,7 @@ Proof using.
   exists h' v. splits~. { subst. applys* red_app_funs_val. }
 Qed.
 
-Lemma rule_apps_fixs : forall xs f F (Vs:vals) t1 H Q,
+Lemma triple_apps_fixs : forall xs f F (Vs:vals) t1 H Q,
   F = (val_fixs f xs t1) ->
   var_fixs f (length Vs) xs ->
   triple (substn (f::xs) (F::Vs) t1) H Q ->
@@ -252,7 +252,7 @@ Qed.
 (* ---------------------------------------------------------------------- *)
 (* ** Rules for loops *)
 
-Lemma rule_while_raw : forall t1 t2 H Q,
+Lemma triple_while_raw : forall t1 t2 H Q,
   triple (trm_if t1 (trm_seq t2 (trm_while t1 t2)) val_unit) H Q ->
   triple (trm_while t1 t2) H Q.
 Proof using.
@@ -260,17 +260,17 @@ Proof using.
   exists h' v. splits~. { applys* red_while. }
 Qed.
 
-Lemma rule_while : forall t1 t2 H Q,
+Lemma triple_while : forall t1 t2 H Q,
   (forall t,
      (forall H' Q', triple (trm_if t1 (trm_seq t2 t) val_unit) H' Q' ->
                     triple t H' Q') ->
     triple t H Q) ->
   triple (trm_while t1 t2) H Q.
 Proof using.
-  introv M. applys M. introv K. applys rule_while_raw. applys K.
+  introv M. applys M. introv K. applys triple_while_raw. applys K.
 Qed.
 
-Lemma rule_while_inv : forall (A:Type) (I:bool->A->hprop) (R:A->A->Prop) t1 t2 H,
+Lemma triple_while_inv : forall (A:Type) (I:bool->A->hprop) (R:A->A->Prop) t1 t2 H,
   let Q := (fun r => \exists Y, I false Y) in
   wf R ->
   (H ==> (\exists b X, I b X) \* \Top) -> (* LATER: replace \top with H' *)
@@ -280,12 +280,12 @@ Lemma rule_while_inv : forall (A:Type) (I:bool->A->hprop) (R:A->A->Prop) t1 t2 H
   triple (trm_while t1 t2) H Q. (* LATER: allow for weakening on Q *)
 Proof using.
   introv WR H0 HX. xchange (rm H0). xpull ;=> b0 X0.
-  rewrite hstar_comm. applys rule_htop_pre. gen b0.
-  induction_wf IH: WR X0. intros. applys rule_while_raw.
+  rewrite hstar_comm. applys triple_htop_pre. gen b0.
+  induction_wf IH: WR X0. intros. applys triple_while_raw.
   applys HX. intros b' X' HR'. applys~ IH.
 Qed.
 
-Lemma rule_for_raw : forall (x:var) (n1 n2:int) t3 H (Q:val->hprop),
+Lemma triple_for_raw : forall (x:var) (n1 n2:int) t3 H (Q:val->hprop),
   triple (
     If (n1 <= n2)
       then (trm_seq (subst1 x n1 t3) (trm_for x (n1+1) n2 t3))
@@ -296,8 +296,8 @@ Proof using.
   exists h' v. splits~. { applys~ red_for. }
 Qed.
 
-(* LATER: simplify proof using rule_for_raw *)
-Lemma rule_for_gt : forall x n1 n2 t3 H Q,
+(* LATER: simplify proof using triple_for_raw *)
+Lemma triple_for_gt : forall x n1 n2 t3 H Q,
   n1 > n2 ->
   H ==> Q val_unit \* \Top ->
   triple (trm_for x n1 n2 t3) H Q.
@@ -307,8 +307,8 @@ Proof using.
   { hhsimpl. hchanges~ M. }
 Qed.
 
-(* LATER: simplify proof using rule_for_raw *)
-Lemma rule_for_le : forall Q1 (x:var) n1 n2 t3 H Q,
+(* LATER: simplify proof using triple_for_raw *)
+Lemma triple_for_le : forall Q1 (x:var) n1 n2 t3 H Q,
   n1 <= n2 ->
   triple (subst1 x n1 t3) H Q1 ->
   (forall v, triple (trm_for x (n1+1) n2 t3) (Q1 v) Q) ->
@@ -321,8 +321,8 @@ Proof using.
   { rewrite <- htop_hstar_htop. hhsimpl. }
 Qed.
 
-(* LATER: simplify proof using rule_for_raw *)
-Lemma rule_for : forall (x:var) (n1 n2:int) t3 H Q,
+(* LATER: simplify proof using triple_for_raw *)
+Lemma triple_for : forall (x:var) (n1 n2:int) t3 H Q,
   (If (n1 <= n2) then
     (exists Q1,
       triple (subst1 x n1 t3) H Q1 /\
@@ -332,12 +332,12 @@ Lemma rule_for : forall (x:var) (n1 n2:int) t3 H Q,
   triple (trm_for x n1 n2 t3) H Q.
 Proof using.
   introv M. case_if.
-  { destruct M. applys* rule_for_le. }
-  { xapplys* rule_for_gt. { math. } hchanges* M. }
+  { destruct M. applys* triple_for_le. }
+  { xapplys* triple_for_gt. { math. } hchanges* M. }
 Qed.
 
-(* LATER: simplify proof using rule_for_raw *)
-Lemma rule_for_inv : forall (I:int->hprop) H' (x:var) n1 n2 t3 H Q,
+(* LATER: simplify proof using triple_for_raw *)
+Lemma triple_for_inv : forall (I:int->hprop) H' (x:var) n1 n2 t3 H Q,
   (n1 <= n2+1) ->
   (H ==> I n1 \* H') ->
   (forall i, n1 <= i <= n2 ->
@@ -348,11 +348,11 @@ Proof using.
   introv N M1 M2 M3. xchange (rm M1). gen N M2.
   induction_wf IH: (wf_upto (n2+1)) n1; intros.
   asserts M4: (triple (trm_for x (n2 + 1)%I n2 t3) (I (n2+1) \* H') Q).
-  { applys rule_for_gt. { math. }
+  { applys triple_for_gt. { math. }
     { hchanges M3. } }
   tests C: (n1 = n2+1).
   { xapplys M4. }
-  { applys rule_for_le.
+  { applys triple_for_le.
     { math. }
     { xapplys M2. { math. } }
     { simpl. xpull ;=> _. tests C': (n1 = n2).
@@ -362,7 +362,7 @@ Qed.
 
 (** Rules for for-loop not in normal form *)
 
-Lemma rule_for_trm : forall (x:var) (t1 t2 t3:trm) H (Q:val->hprop) (Q1:val->hprop),
+Lemma triple_for_trm : forall (x:var) (t1 t2 t3:trm) H (Q:val->hprop) (Q1:val->hprop),
   triple t1 H Q1 ->
   (forall v1, exists Q2,
       triple t2 (Q1 v1) Q2
@@ -383,7 +383,7 @@ Definition is_val_int (v:val) :=
   exists n, v = val_int n.
 
 (* full rule, too complex *)
-Lemma rule_for_trm_int : forall (x:var) (t1 t2 t3:trm) H (Q:val->hprop) (Q1:val->hprop),
+Lemma triple_for_trm_int : forall (x:var) (t1 t2 t3:trm) H (Q:val->hprop) (Q1:val->hprop),
   triple t1 H Q1 ->
   (forall v, ~ is_val_int v -> (Q1 v) ==> \[False]) ->
   (forall (n1:int), exists Q2,
@@ -391,7 +391,7 @@ Lemma rule_for_trm_int : forall (x:var) (t1 t2 t3:trm) H (Q:val->hprop) (Q1:val-
    /\ (forall v, ~ is_val_int v -> (Q2 v) ==> \[False])
    /\ (forall (n2:int), triple (trm_for x n1 n2 t3) (Q2 (val_int n2)) Q)) ->
   triple (trm_for x t1 t2 t3) H Q.
-Proof using. (* might be simplified using rule_for_trm *)
+Proof using. (* might be simplified using triple_for_trm *)
   introv M1 nQ1 M2. intros HF h Hf. forwards (h1'&v1&R1&K1): (rm M1) Hf.
   tests C1: (is_val_int v1).
   { destruct C1 as (n1&E). subst. lets (Q2&M2'&nQ2&M3): ((rm M2) n1).
@@ -422,7 +422,7 @@ Qed.
 Section RulesStateOps.
 Transparent hstar hsingle hfield hexists loc null.
 
-Lemma rule_ref : forall v,
+Lemma triple_ref : forall v,
   triple (val_ref v)
     \[]
     (fun r => \exists l, \[r = val_loc l] \* l ~~~> v).
@@ -437,7 +437,7 @@ Proof using.
     { splits~. hhsimpl~. } }
 Qed.
 
-Lemma rule_get : forall v l,
+Lemma triple_get : forall v l,
   triple (val_get (val_loc l))
     (l ~~~> v)
     (fun x => \[x = v] \* (l ~~~> v)).
@@ -448,7 +448,7 @@ Proof using.
   { rew_heap. rewrite hstar_pure. split~. hhsimpl~. }
 Qed.
 
-Lemma rule_set : forall w l v,
+Lemma triple_set : forall w l v,
   triple (val_set (val_loc l) w)
     (l ~~~> v)
     (fun r => \[r = val_unit] \* l ~~~> w).
@@ -463,17 +463,17 @@ Proof using.
     { subst h1. applys~ fmap_disjoint_single_set v. } }
 Qed.
 
-Lemma rule_set' : forall w l v,
+Lemma triple_set' : forall w l v,
   triple (val_set (val_loc l) w)
     (l ~~~> v)
     (fun r => l ~~~> w).
-Proof using. intros. xapplys* rule_set. Qed.
+Proof using. intros. xapplys* triple_set. Qed.
 
 
 (* ---------------------------------------------------------------------- *)
 (** Alloc function *)
 
-Lemma rule_alloc : forall n,
+Lemma triple_alloc : forall n,
   n >= 0 ->
   triple (val_alloc n)
     \[]
@@ -496,7 +496,7 @@ End RulesStateOps.
 (* ---------------------------------------------------------------------- *)
 (** Other primitive functions *)
 
-Lemma rule_eq : forall v1 v2,
+Lemma triple_eq : forall v1 v2,
   triple (val_eq v1 v2)
     \[]
     (fun r => \[r = isTrue (v1 = v2)]).
@@ -506,7 +506,7 @@ Proof using.
   { hhsimpl~. }
 Qed.
 
-Lemma rule_add : forall n1 n2,
+Lemma triple_add : forall n1 n2,
   triple (val_add n1 n2)
     \[]
     (fun r => \[r = val_int (n1 + n2)]).
@@ -516,7 +516,7 @@ Proof using.
   { hhsimpl*. }
 Qed.
 
-Lemma rule_sub : forall n1 n2,
+Lemma triple_sub : forall n1 n2,
   triple (val_sub n1 n2)
     \[]
     (fun r => \[r = val_int (n1 - n2)]).
@@ -526,7 +526,7 @@ Proof using.
   { hhsimpl*. }
 Qed.
 
-Lemma rule_ptr_add : forall l n,
+Lemma triple_ptr_add : forall l n,
   l + n >= 0 ->
   triple (val_ptr_add l n)
     \[]
@@ -537,19 +537,19 @@ Proof using.
   { hhsimpl*. }
 Qed.
 
-Lemma rule_ptr_add_nat : forall l (f:nat),
+Lemma triple_ptr_add_nat : forall l (f:nat),
   triple (val_ptr_add l f)
     \[]
     (fun r => \[r = val_loc (l+f)%nat]).
 Proof using.
-  intros. xapplys~ rule_ptr_add. { math. }
+  intros. xapplys~ triple_ptr_add. { math. }
   { intros. subst. fequals.
     applys eq_nat_of_eq_int. rewrite abs_nonneg; math. }
 Qed.
 
-(** Alternative direct proof for [rule_ptr_add_nat] *)
+(** Alternative direct proof for [triple_ptr_add_nat] *)
 
-Lemma rule_ptr_add_nat' : forall l (f:nat),
+Lemma triple_ptr_add_nat' : forall l (f:nat),
   triple (val_ptr_add l f)
     \[]
     (fun r => \[r = val_loc (l+f)%nat]).
@@ -567,54 +567,54 @@ Qed.
 (* ---------------------------------------------------------------------- *)
 (* ** Practical additional rules *)
 
-(** Combination of [rule_val] and [rule_htop_post] *)
+(** Combination of [triple_val] and [triple_htop_post] *)
 
-Lemma rule_val_htop : forall v H Q,
+Lemma triple_val_htop : forall v H Q,
   H ==> Q v \* \Top ->
   triple (trm_val v) H Q.
 Proof using.
-  introv M. applys rule_htop_post. applys~ rule_val.
+  introv M. applys triple_htop_post. applys~ triple_val.
 Qed.
 
-(** Combination of [rule_frame] and [rule_conseq] *)
+(** Combination of [triple_frame] and [triple_conseq] *)
 
-Lemma rule_frame_consequence : forall H2 H1 Q1 t H Q,
+Lemma triple_frame_consequence : forall H2 H1 Q1 t H Q,
   H ==> H1 \* H2 ->
   triple t H1 Q1 ->
   Q1 \*+ H2 ===> Q ->
   triple t H Q.
 Proof using.
-  introv WH M WQ. applys rule_conseq WH WQ. applys rule_frame M.
+  introv WH M WQ. applys triple_conseq WH WQ. applys triple_frame M.
 Qed.
 
-(** Combination of [rule_let] and [rule_val] *)
+(** Combination of [triple_let] and [triple_val] *)
 
-Lemma rule_let_val : forall z v1 t2 H Q,
+Lemma triple_let_val : forall z v1 t2 H Q,
   (forall (X:val), X = v1 -> triple (subst1 z X t2) H Q) ->
   triple (trm_let z (trm_val v1) t2) H Q.
 Proof using.
   introv M. forwards~ M': (rm M).
-  applys_eq~ (>> rule_let H (fun x => \[x = v1] \* H)) 2.
-  { applys rule_val. hsimpl~. }
-  { intros X. applys rule_extract_hprop. intro_subst. applys M'. }
+  applys_eq~ (>> triple_let H (fun x => \[x = v1] \* H)) 2.
+  { applys triple_val. hsimpl~. }
+  { intros X. applys triple_extract_hprop. intro_subst. applys M'. }
 Qed.
 
 (** A rule of conditionals with case analysis already done *)
 
-Lemma rule_if' : forall Q1 t0 t1 t2 H Q,
+Lemma triple_if' : forall Q1 t0 t1 t2 H Q,
   triple t0 H Q1 ->
   triple t1 (Q1 true) Q ->
   triple t2 (Q1 false) Q ->
   (forall v, ~ is_val_bool v -> (Q1 v) ==> \[False]) ->
   triple (trm_if t0 t1 t2) H Q.
 Proof using.
-  introv M1 M2 M3 M4. applys* rule_if.
+  introv M1 M2 M3 M4. applys* triple_if.
   { intros b. case_if*. }
 Qed.
 
-(** A direct proof for [rule_if_bool] *)
+(** A direct proof for [triple_if_bool] *)
 
-Lemma rule_if_bool' : forall v t1 t2 H Q,
+Lemma triple_if_bool' : forall v t1 t2 H Q,
   (v = true -> triple t1 H Q) ->
   (v = false -> triple t2 H Q) ->
   (is_val_bool v) ->
@@ -632,7 +632,7 @@ Qed.
 
 (** A rule for unary function application *)
 
-Lemma rule_app : forall (f:bind) x F V t1 H Q,
+Lemma triple_app : forall (f:bind) x F V t1 H Q,
   F = (val_fix f x t1) ->
   triple (subst2 f F x V t1) H Q ->
   triple (trm_app F V) H Q.
