theories/SLRules.v
@@ -52,7 +52,7 @@ Require Import LambdaSemantics LambdaSep.
 
 
 (* Note: specialized version of consequence *)
-Lemma rule_htop_post_remove : forall t H Q,
+Lemma triple_htop_post_remove : forall t H Q,
   triple t H Q ->
   triple t H (Q \*+ \Top).
 Proof using.
@@ -63,3 +63,14 @@ Qed.
 
 
 
+
+
+Lemma Triple_seq : forall t1 t2 H,
+  forall A `{EA:Enc A} (Q:A->hprop) (Q1:unit->hprop),
+  Triple t1 H Q1 ->
+  Triple t2 (Q1 tt) Q ->
+  Triple (trm_seq t1 t2) H Q.
+Proof using.
+
+  introv M1 M2. applys* Triple_let M1. intros X.
+  unfold Subst1. rewrite subst1_anon. destruct X. applys M2.
